Overall update of deriv notations

nola/deriv.v
@@ -2,42 +2,62 @@
 
 From nola Require Export util.pred util.wft.
 
+(** [dwrap]: Wrapper for derivability *)
+#[projections(primitive)]
+Record dwrap (A : Type) := Dwrap { dunwrap : A }.
+Arguments Dwrap {_} _.
+Arguments dunwrap {_} _.
+Add Printing Constructor dwrap.
+
 (** ** [judg]: Judgment information *)
 #[projections(primitive)]
-Structure judg := Judg {
+Record judg := Judg {
   (** Index type, with a well-founded relation *)
-  #[canonical=no] judg_idx : wft;
+  judg_idx : wft;
   (** Data type *)
-  judg_data :> judg_idx → Type;
+  judg_data : judg_idx → Type;
   (** Semantics *)
-  #[canonical=no] judg_sem :
-    (∀ i, judg_data i → Prop) → ∀ i, judg_data i → Prop;
+  judg_sem : dwrap (∀ i, judg_data i → Prop) → ∀ i, judg_data i → Prop;
 }.
 Add Printing Constructor judg.
 Arguments judg_sem {JU} d i J : rename.
 
 (** Derivability predicate *)
-Notation deriv_ty JU := (∀ i, JU.(judg_data) i → Prop).
+Notation deriv_ty JU := (dwrap (∀ i, JU.(judg_data) i → Prop)).
 (** Derivability predicate parameterized over a derivability predicate *)
 Notation pderiv_ty JU := (deriv_ty JU → deriv_ty JU).
 
+(** Modified [judg_sem] *)
+Notation judg_sem' d := (Dwrap (judg_sem d)).
+
+(** Notation for derivability *)
+Module DerivNotation.
+  Notation "⊢{ d , i }" := (dunwrap d i) (format "⊢{ d ,  i }") : nola_scope.
+  Notation "⊨{ d , i }" := (judg_sem d i) (format "⊨{ d ,  i }")
+    : nola_scope.
+  Notation "⟦ d ⟧ᵈ" := (judg_sem' d) (format "⟦ d ⟧ᵈ") : nola_scope.
+End DerivNotation.
+Import DerivNotation.
+
 (** Operations on derivability predicates *)
 
-Definition Falseᵈ {JU} : deriv_ty JU := λ _ _, False.
+Definition Falseᵈ {JU} : deriv_ty JU := Dwrap (λ _ _, False).
 Notation "⊥ᵈ" := Falseᵈ : nola_scope.
 
-Definition orᵈ {JU} (d d' : deriv_ty JU) : deriv_ty JU := λ i J, d i J ∨ d' i J.
+Definition orᵈ {JU} (d d' : deriv_ty JU) : deriv_ty JU :=
+  Dwrap (λ i J, ⊢{d,i} J ∨ ⊢{d',i} J).
 Infix "∨ᵈ" := orᵈ (at level 50, left associativity) : nola_scope.
 
 Definition apporᵈ {JU} (δ : pderiv_ty JU) (d : deriv_ty JU) : deriv_ty JU :=
   δ d ∨ᵈ d.
 Infix "$∨ᵈ" := apporᵈ (at level 50, left associativity) : nola_scope.
 
-Definition implᵈ {JU} (d d' : deriv_ty JU) : Prop := ∀ i J, d i J → d' i J.
+Definition implᵈ {JU} (d d' : deriv_ty JU) : Prop :=
+  ∀ i J, ⊢{d,i} J → ⊢{d',i} J.
 Infix "→ᵈ" := implᵈ (at level 99, right associativity) : nola_scope.
 
 Definition implᵈ_low {JU} (i : JU.(judg_idx)) (d d' : deriv_ty JU) : Prop :=
-  ∀ j, j ≺ i → ∀ K, d j K → d' j K.
+  ∀ j, j ≺ i → ∀ K, ⊢{d,j} K → ⊢{d',j} K.
 Infix "→ᵈ[≺ i ]" := (implᵈ_low i) (at level 99, right associativity)
   : nola_scope.
 
@@ -50,11 +70,11 @@ Record derivy_gen (JU : judg) (self : pderiv_ty JU → Prop) (δ : pderiv_ty JU)
   derivy_gen_mono {d d' : deriv_ty JU} : (d →ᵈ d') → δ d →ᵈ δ d';
   (** [δ] can accumulate coinductive hypotheses *)
   derivy_gen_acc {d} (res : deriv_ty JU) : (res →ᵈ δ (d ∨ᵈ res)) → res →ᵈ δ d;
-  (** [δ d i J] can be proved by semantics *)
+  (** [⊢{δ d, i} J] can be proved by semantics *)
   derivy_gen_bysem {d i J} :
-    (∀ δ', self δ' → (δ d i →₁ judg_sem (δ' ⊥ᵈ) i) → (δ $∨ᵈ d →ᵈ δ' ⊥ᵈ) →
-      (δ' ⊥ᵈ →ᵈ[≺ i] judg_sem (δ' ⊥ᵈ)) → judg_sem (δ' ⊥ᵈ) i J) →
-    δ d i J
+    (∀ δ', self δ' → (⊢{δ d, i} →₁ ⊨{δ' ⊥ᵈ, i}) → (δ $∨ᵈ d →ᵈ δ' ⊥ᵈ) →
+      (δ' ⊥ᵈ →ᵈ[≺ i] ⟦δ' ⊥ᵈ⟧ᵈ) → ⊨{δ' ⊥ᵈ, i} J) →
+    ⊢{δ d, i} J
 }.
 #[export] Instance derivy_gen_mono₁₁ {JU} : Mono₁₁ (derivy_gen JU).
 Proof.
@@ -72,12 +92,12 @@ Class inderivy (JU : judg) (δ' δ : pderiv_ty JU) (d : deriv_ty JU)
   (i : JU.(judg_idx)) : Prop := {
   (** [δ'] satisfies [derivy] *)
   inderivy_derivy :: derivy JU δ';
-  (** Interpret [δ d i] as [judg_sem (δ' ⊥ᵈ) i] *)
-  inderivy_sem : δ d i →₁ judg_sem (δ' ⊥ᵈ) i;
+  (** Interpret [⊢{δ d, i}] as [⊨{δ' ⊥ᵈ, i}] *)
+  inderivy_sem : ⊢{δ d, i} →₁ ⊨{δ' ⊥ᵈ, i};
   (** Turn [δ $∨ᵈ d] into [δ' ⊥ᵈ] *)
   inderivy_turn : δ $∨ᵈ d →ᵈ δ' ⊥ᵈ;
-  (** Interpret [δ' ⊥ᵈ j] as [judg_sem (δ' ⊥ᵈ) j] for [j ≺ i] *)
-  inderivy_semlow : δ' ⊥ᵈ →ᵈ[≺ i] judg_sem (δ' ⊥ᵈ);
+  (** Interpret [⊢{δ' ⊥ᵈ, j}] as [⊨{δ' ⊥ᵈ, j}] for [j ≺ i] *)
+  inderivy_semlow : δ' ⊥ᵈ →ᵈ[≺ i] ⟦δ' ⊥ᵈ⟧ᵈ;
 }.
 
 (** Lemmas for [derivy] *)
@@ -87,7 +107,7 @@ Lemma derivy_acc `{D : derivy JU δ} {d} res :
   (res →ᵈ δ (d ∨ᵈ res)) → res →ᵈ δ d.
 Proof. move: D=> /mu_unfold [_ acc _]. apply acc. Qed.
 Lemma derivy_bysem `{D : derivy JU δ} {d i J} :
-  (∀ δ', inderivy JU δ' δ d i → judg_sem (δ' ⊥ᵈ) i J) → δ d i J.
+  (∀ δ', inderivy JU δ' δ d i → ⊨{δ' ⊥ᵈ, i} J) → ⊢{δ d, i} J.
 Proof. move: D=> /mu_unfold [_ _ bysem]=> H. apply bysem=> *. by apply H. Qed.
 
 (** Lemmas for [inderivy] *)
@@ -95,43 +115,41 @@ Lemma inderivy_turn_l `{!inderivy JU δ' δ d i} : δ d →ᵈ δ' ⊥ᵈ.
 Proof. move=> *. apply inderivy_turn. by left. Qed.
 Lemma inderivy_turn_r `{!inderivy JU δ' δ d i} : d →ᵈ δ' ⊥ᵈ.
 Proof. move=> *. apply inderivy_turn. by right. Qed.
-Lemma inderivy_turn_semlow `{!inderivy JU δ' δ d i} :
-  δ $∨ᵈ d →ᵈ[≺ i] judg_sem (δ' ⊥ᵈ).
-Proof. move=> *. apply inderivy_semlow; by [|apply inderivy_turn]. Qed.
-Lemma inderivy_turn_semlow_l `{!inderivy JU δ' δ d i} :
-  δ d →ᵈ[≺ i] judg_sem (δ' ⊥ᵈ).
-Proof. move=> *. apply inderivy_turn_semlow; by [|left]. Qed.
-Lemma inderivy_turn_semlow_r `{!inderivy JU δ' δ d i} :
-  d →ᵈ[≺ i] judg_sem (δ' ⊥ᵈ).
-Proof. move=> *. apply inderivy_turn_semlow; by [|right]. Qed.
+Lemma inderivy_turn_semlow `{!inderivy JU δ' δ d i} : δ $∨ᵈ d →ᵈ[≺ i] ⟦δ' ⊥ᵈ⟧ᵈ.
+Proof. move=>/= *. apply inderivy_semlow; by [|apply inderivy_turn]. Qed.
+Lemma inderivy_turn_semlow_l `{!inderivy JU δ' δ d i} :  δ d →ᵈ[≺ i] ⟦δ' ⊥ᵈ⟧ᵈ.
+Proof. move=>/= *. apply inderivy_turn_semlow; by [|left]. Qed.
+Lemma inderivy_turn_semlow_r `{!inderivy JU δ' δ d i} : d →ᵈ[≺ i] ⟦δ' ⊥ᵈ⟧ᵈ.
+Proof. move=>/= *. apply inderivy_turn_semlow; by [|right]. Qed.
 
 (** ** [deriv]: Derivability *)
 
 (** Generator of [deriv] *)
-Inductive deriv_gen (JU : judg) (self : deriv_ty JU) i (J : JU i) : Prop := {
+Inductive deriv_gen (JU : judg) (self : deriv_ty JU) i
+  (J : JU.(judg_data) i) : Prop := {
   (* Parameterization by [deriv_i] serves for strict positivity *)
   deriv_gen_bysem : ∃ deriv_i, (deriv_i →₁ deriv_gen JU self i) ∧
-    (∀ δ', derivy JU δ' → (deriv_i →₁ judg_sem (δ' ⊥ᵈ) i) → (self →ᵈ δ' ⊥ᵈ) →
-      (δ' ⊥ᵈ →ᵈ[≺ i] judg_sem (δ' ⊥ᵈ)) → judg_sem (δ' ⊥ᵈ) i J)
+    (∀ δ', derivy JU δ' → (deriv_i →₁ ⊨{δ' ⊥ᵈ, i}) → (self →ᵈ δ' ⊥ᵈ) →
+      (δ' ⊥ᵈ →ᵈ[≺ i] ⟦δ' ⊥ᵈ⟧ᵈ) → ⊨{δ' ⊥ᵈ, i} J)
 }.
 
 (** Argument data of [deriv_ty JU] *)
 #[projections(primitive)]
 Record deriv_aty (JU : judg) := DerivAty {
   deriv_aty_idx : JU.(judg_idx);
-  deriv_aty_data : JU deriv_aty_idx;
+  deriv_aty_data : JU.(judg_data) deriv_aty_idx;
 }.
 Arguments DerivAty {_} _ _.
 
 (** Conversion between [deriv_aty JU → Prop] and [deriv_ty JU] *)
 Definition deriv_curry {JU} (d : deriv_aty JU → Prop) : deriv_ty JU :=
-  λ i J, d (DerivAty i J).
+  Dwrap (λ i J, d (DerivAty i J)).
 Definition deriv_uncurry {JU} (d : deriv_ty JU) : deriv_aty JU → Prop :=
-  λ '(DerivAty i J), d i J.
+  λ '(DerivAty i J), ⊢{d,i} J.
 
 (** Modified [deriv_gen] *)
 Definition deriv_gen' JU (d : deriv_aty JU → Prop) : deriv_aty JU → Prop :=
-  deriv_uncurry (deriv_gen JU (deriv_curry d)).
+  deriv_uncurry (Dwrap (deriv_gen JU (deriv_curry d))).
 #[export] Instance deriv_gen'_mono JU : Mono₁₁ (deriv_gen' JU).
 Proof.
   move=> d d' dd' [i J] +. move: i J. fix FIX 3=> i J [[der[derto big]]].
@@ -150,14 +168,14 @@ Proof.
   - move=> d d' dd' i J. apply pnu_mono=> [[j K]] /dd'. done.
   - move=> d res resto i J ?. apply (pnu_acc (deriv_uncurry res)); [|done].
     move=> [j K] /resto. done.
-  - move=> d i J H. apply pnu_fold. split. exists (deriv JU d i).
+  - move=> d i J H. apply pnu_fold. split. exists ⊢{deriv JU d, i}.
     split. { by move=> J' /pnu_unfold. } { move=> δ'. apply H. }
 Qed.
 
 (** Soundness of [deriv] *)
-Lemma deriv_sound {JU} : deriv JU ⊥ᵈ →ᵈ judg_sem (deriv JU ⊥ᵈ).
+Lemma deriv_sound {JU} : deriv JU ⊥ᵈ →ᵈ ⟦deriv JU ⊥ᵈ⟧ᵈ.
 Proof.
-  move=> i +. elim: {i}(wft_lt_wf i)=> i _ IH + /nu_unfold. fix FIX 2.
+  move=>/= i +. elim: {i}(wft_lt_wf i)=> i _ IH + /nu_unfold. fix FIX 2.
   move=> J [[drvi[drvito big]]]. apply big. { apply _. }
   { move=> J' /drvito. apply FIX. } { by move=> *. } { done. }
 Qed.
