nola/examples/logic/deriv.v
@@ -9,9 +9,8 @@ Implicit Type (d : nderiv_ty) (δ : npderiv_ty) (i j : nat).
 (** ** Basic notions *)
 
 (** [nJudg]: Judgment *)
-Definition nJudgTy i : Type := nPropL (;ᵞ) * nPropL (;ᵞ).
-Canonical nJudg Σ `{!nintpG Σ} := Judg nat nJudgTy
-  (λ d _ '(P, Q), ⟦ P ⟧(d) ⊢ ⟦ Q ⟧(d)).
+Definition nJudg Σ `{!nintpG Σ} : judg :=
+  Judg nat (λ _, nJudgT) (λ d _ '(njudg P Q), ⟦ P ⟧(d) ⊢ ⟦ Q ⟧(d)).
 
 (** *[nderivy], [ninderivy], [nderiv]: Derivability *)
 Class nderivy Σ `{!nintpG Σ} δ := Nderivy {
@@ -27,13 +26,14 @@ Class ninderivy Σ `{!nintpG Σ} δ δ' d i := Ninderivy {
 Definition nderiv Σ `{!nintpG Σ} : npderiv_ty := deriv (nJudg Σ).
 
 (** Operations on [nderiv_ty] *)
-Definition Falseⁿᵈ : nderiv_ty := λ _ _, False.
+Definition Falseⁿᵈ : nderiv_ty := Dwrap (λ _ _, False).
 Notation "⊥ⁿᵈ" := Falseⁿᵈ : nola_scope.
-Definition orⁿᵈ d d' : nderiv_ty := λ i PQ, d i PQ ∨ d' i PQ.
+Definition orⁿᵈ d d' : nderiv_ty :=
+  Dwrap (λ i '(njudg P Q), (P ⊢{d,i} Q) ∨ (P ⊢{d',i} Q)).
 Infix "∨ⁿᵈ" := orⁿᵈ (at level 50, left associativity) : nola_scope.
 Definition apporⁿᵈ δ d : nderiv_ty := δ d ∨ⁿᵈ d.
 Infix "$∨ⁿᵈ" := apporⁿᵈ (at level 50, left associativity) : nola_scope.
-Definition implⁿᵈ d d' : Prop := ∀ i PQ, d i PQ → d' i PQ.
+Definition implⁿᵈ d d' : Prop := ∀ i P Q, (P ⊢{d,i} Q) → P ⊢{d',i} Q.
 Infix "→ⁿᵈ" := implⁿᵈ (at level 99, right associativity) : nola_scope.
 
 (** ** Lemmas *)
@@ -44,49 +44,54 @@ Section basic.
 
   (** [δ] is monotone over the coinductive hypothesis *)
   Lemma n_mono {d d'} : (d →ⁿᵈ d') → δ d →ⁿᵈ δ d'.
-  Proof. apply (derivy_mono (JU:=nJudg Σ)). Qed.
+  Proof.
+    move=> dd' ???. apply (derivy_mono (JU:=nJudg Σ))=>/= ?[??]. apply dd'.
+  Qed.
 
   (** [δ] can accumulate the coinductive hypothesis *)
   Lemma n_acc {d} res : (res →ⁿᵈ δ (d ∨ⁿᵈ res)) → res →ⁿᵈ δ d.
-  Proof. apply (derivy_acc (JU:=nJudg Σ)). Qed.
+  Proof.
+    move=> resto ???. apply (derivy_acc (JU:=nJudg Σ))=> ?[??]. by apply resto.
+  Qed.
 
   (** [δ] can be proved by its semantics *)
   Lemma n_bysem {d i P Q} :
     (∀ δ', ninderivy Σ δ' δ d i → ⟦ P ⟧(δ' ⊥ⁿᵈ) ⊢ ⟦ Q ⟧(δ' ⊥ⁿᵈ)) →
-    δ d i (P, Q).
+    P ⊢{δ d, i} Q.
   Proof. move=> H. apply (derivy_bysem (JU:=nJudg Σ))=> ??. by apply H. Qed.
 
-  (** We can get [⊢] out of [δ] under [ninderivy Σ δ' δ] *)
+  (** We can get Iris [⊢] out of [⊢{δ d, i}] under [ninderivy Σ δ' δ] *)
   Lemma nin_sem {δ' : npderiv_ty} `{!ninderivy Σ δ' δ d i} {P Q} :
-    δ d i (P, Q) → ⟦ P ⟧(δ' ⊥ⁿᵈ) ⊢ ⟦ Q ⟧(δ' ⊥ⁿᵈ).
-  Proof. apply (inderivy_sem (JU:=nJudg Σ) (P, Q)). Qed.
+    P ⊢{δ d, i} Q → ⟦ P ⟧(δ' ⊥ⁿᵈ) ⊢ ⟦ Q ⟧(δ' ⊥ⁿᵈ).
+  Proof. apply (inderivy_sem (JU:=nJudg Σ)). Qed.
 
   (** We can turn [δ $∨ⁿᵈ d] into [δ' ⊥ⁿᵈ] under [ninderivy] *)
-  Lemma nin_turn `{!ninderivy Σ δ' δ d i} : (δ $∨ⁿᵈ d) →ⁿᵈ δ' ⊥ⁿᵈ.
-  Proof. apply (inderivy_turn (JU:=nJudg Σ)). Qed.
+  Lemma nin_turn `{!ninderivy Σ δ' δ d i} : δ $∨ⁿᵈ d →ⁿᵈ δ' ⊥ⁿᵈ.
+  Proof. move=> ???. apply (inderivy_turn (JU:=nJudg Σ)). Qed.
 
-  (** We can get [⊢] out of [δ' j] for [j < i] under [ninderivy Σ δ' δ d i] *)
+  (** We can get Iris [⊢] out of [⊢{δ', j}] for [j < i]
+    under [ninderivy Σ δ' δ d i] *)
   Lemma nin_semlow `{!ninderivy Σ δ' δ d i} {j P Q} :
-    j < i → δ' ⊥ⁿᵈ j (P, Q) → ⟦ P ⟧(δ' ⊥ⁿᵈ) ⊢ ⟦ Q ⟧(δ' ⊥ⁿᵈ).
-  Proof. move=> ji H. apply (inderivy_semlow (JU:=nJudg Σ) j ji (P, Q) H). Qed.
+    j < i → P ⊢{δ' ⊥ⁿᵈ, j} Q → ⟦ P ⟧(δ' ⊥ⁿᵈ) ⊢ ⟦ Q ⟧(δ' ⊥ⁿᵈ).
+  Proof. move=> ji PQ. apply (inderivy_semlow (JU:=nJudg Σ) _ ji _ PQ). Qed.
 
   (** Utility lemmas *)
   Lemma nin_turn_l `{!ninderivy Σ δ' δ d i} : δ d →ⁿᵈ δ' ⊥ⁿᵈ.
-  Proof. apply (inderivy_turn_l (JU:=nJudg Σ)). Qed.
+  Proof. move=> *. apply nin_turn. by left. Qed.
   Lemma nin_turn_r `{!ninderivy Σ δ' δ d i} : d →ⁿᵈ δ' ⊥ⁿᵈ.
-  Proof. apply (inderivy_turn_r (JU:=nJudg Σ)). Qed.
+  Proof. move=> *. apply nin_turn. by right. Qed.
   Lemma nin_turn_semlow `{!ninderivy Σ δ' δ d i} {j P Q} :
-    j < i → (δ $∨ⁿᵈ d) j (P, Q) → ⟦ P ⟧(δ' ⊥ⁿᵈ) ⊢ ⟦ Q ⟧(δ' ⊥ⁿᵈ).
+    j < i → P ⊢{δ $∨ⁿᵈ d, j} Q → ⟦ P ⟧(δ' ⊥ⁿᵈ) ⊢ ⟦ Q ⟧(δ' ⊥ⁿᵈ).
   Proof. move=> ji ?. by apply (nin_semlow ji), nin_turn. Qed.
   Lemma nin_turn_semlow_l `{!ninderivy Σ δ' δ d i} {j P Q} :
-    j < i → δ d j (P, Q) → ⟦ P ⟧(δ' ⊥ⁿᵈ) ⊢ ⟦ Q ⟧(δ' ⊥ⁿᵈ).
+    j < i → P ⊢{δ d, j} Q → ⟦ P ⟧(δ' ⊥ⁿᵈ) ⊢ ⟦ Q ⟧(δ' ⊥ⁿᵈ).
   Proof. move=> ji ?. by apply (nin_semlow ji), nin_turn_l. Qed.
   Lemma nin_turn_semlow_r `{!ninderivy Σ δ' δ d i} {j P Q} :
-    j < i → d j (P, Q) → ⟦ P ⟧(δ' ⊥ⁿᵈ) ⊢ ⟦ Q ⟧(δ' ⊥ⁿᵈ).
+    j < i → P ⊢{d, j} Q → ⟦ P ⟧(δ' ⊥ⁿᵈ) ⊢ ⟦ Q ⟧(δ' ⊥ⁿᵈ).
   Proof. move=> ji ?. by apply (nin_semlow ji), nin_turn_r. Qed.
 
-  (** [δ] is monotone over the index *)
-  Lemma n_up {i j d P Q} : i ≤ j → δ d i (P, Q) → δ d j (P, Q).
+  (** [δ d] is monotone over the index *)
+  Lemma n_up {i j d P Q} : i ≤ j → P ⊢{δ d, i} Q → P ⊢{δ d, j} Q.
   Proof.
     move=> /Nat.lt_eq_cases [|<-]; [|done]=> ? H. apply n_bysem=> ??.
     by apply nin_turn_semlow_l in H.
@@ -102,6 +107,6 @@ Section nderiv.
 
   (** [nderiv] is sound *)
   Lemma nderiv_sound {i P Q} :
-    nderiv Σ ⊥ⁿᵈ i (P, Q) → ⟦ P ⟧(nderiv Σ ⊥ⁿᵈ) ⊢ ⟦ Q ⟧(nderiv Σ ⊥ⁿᵈ).
-  Proof. exact (deriv_sound (JU:=nJudg Σ) i (P, Q)). Qed.
+    P ⊢{nderiv Σ ⊥ⁿᵈ, i} Q → ⟦ P ⟧(nderiv Σ ⊥ⁿᵈ) ⊢ ⟦ Q ⟧(nderiv Σ ⊥ⁿᵈ).
+  Proof. apply (deriv_sound (JU:=nJudg Σ)). Qed.
 End nderiv.
