nola/examples/logic/facts.v
@@ -10,255 +10,254 @@ Section bi.
   Context `{!nintpG Σ, !nderivy Σ δ}.
 
   (** [δ] is reflexive *)
-  Lemma n_refl {d i P} : δ d i (P, P).
+  Lemma n_refl {d i P} : P ⊢{δ d, i} P.
   Proof. by apply n_bysem. Qed.
 
   (** [δ] is transitive *)
-  Lemma n_trans {d i P Q R} : δ d i (P, Q) → δ d i (Q, R) → δ d i (P, R).
+  Lemma n_trans {d i P Q R} : P ⊢{δ d, i} Q → Q ⊢{δ d, i} R → P ⊢{δ d, i} R.
   Proof.
     move=> H H'. apply n_bysem=> >. by move: H H'=> /nin_sem-> /nin_sem->.
   Qed.
 
   (** Laws for [⌜_⌝] *)
-  Lemma n_pure_intro {d i} {φ : Prop} {P} : φ → δ d i (P, ⌜φ⌝)%n.
+  Lemma n_pure_intro {d i} {φ : Prop} {P} : φ → P ⊢{δ d, i} ⌜φ⌝.
   Proof. move=> ?. apply n_bysem=>/= >. by apply bi.pure_intro. Qed.
   Lemma n_pure_elim {d i} {φ : Prop} {P} :
-    (φ → δ d i (True, P)%n) → δ d i (⌜φ⌝, P)%n.
+    (φ → True ⊢{δ d, i} P) → ⌜φ⌝ ⊢{δ d, i} P.
   Proof.
     move=> H. apply n_bysem=>/= >. apply (bi.pure_elim φ); [done|]=> x.
     move: (H x)=> /nin_sem/= <-. apply bi.True_intro.
   Qed.
 
   (** Laws for [∧] *)
-  Lemma n_and_elim_l {d i P Q} : δ d i (P ∧ Q, P)%n.
+  Lemma n_and_elim_l {d i P Q} : P ∧ Q ⊢{δ d, i} P.
   Proof. apply n_bysem=>/= >. by apply bi.and_elim_l. Qed.
-  Lemma n_and_elim_r {d i P Q} : δ d i (P ∧ Q, Q)%n.
+  Lemma n_and_elim_r {d i P Q} : P ∧ Q ⊢{δ d, i} Q.
   Proof. apply n_bysem=>/= >. by apply bi.and_elim_r. Qed.
   Lemma n_and_intro {d i P Q R} :
-    δ d i (P, Q) → δ d i (P, R)%n → δ d i (P, Q ∧ R)%n.
+    P ⊢{δ d, i} Q → P ⊢{δ d, i} R → P ⊢{δ d, i} Q ∧ R.
   Proof.
     move=> ??. apply n_bysem=>/= >. by apply bi.and_intro; apply nin_sem.
   Qed.
 
   (** Laws for [∨] *)
-  Lemma n_or_intro_l {d i P Q} : δ d i (P, P ∨ Q)%n.
+  Lemma n_or_intro_l {d i P Q} : P ⊢{δ d, i} P ∨ Q.
   Proof. apply n_bysem=>/= >. by apply bi.or_intro_l. Qed.
-  Lemma n_or_intro_r {d i P Q} : δ d i (Q, P ∨ Q)%n.
+  Lemma n_or_intro_r {d i P Q} : Q ⊢{δ d, i} P ∨ Q.
   Proof. apply n_bysem=>/= >. by apply bi.or_intro_r. Qed.
   Lemma n_or_elim {d i P Q R} :
-    δ d i (P, R)%n → δ d i (Q, R)%n → δ d i (P ∨ Q, R)%n.
+    P ⊢{δ d, i} R → Q ⊢{δ d, i} R → P ∨ Q ⊢{δ d, i} R.
   Proof.
     move=> ??. apply n_bysem=>/= >. by apply bi.or_elim; apply nin_sem.
   Qed.
 
   (** Laws for [→] *)
-  Lemma n_impl_intro_r {d i P Q R} : δ d i (P ∧ Q, R)%n → δ d i (P, Q → R)%n.
+  Lemma n_impl_intro_r {d i P Q R} : P ∧ Q ⊢{δ d, i} R → P ⊢{δ d, i} (Q → R).
   Proof.
     move=> H. apply n_bysem=>/= >. apply bi.impl_intro_r. by apply nin_sem in H.
   Qed.
-  Lemma n_impl_elim_l' {d i P Q R} : δ d i (P, Q → R)%n → δ d i (P ∧ Q, R)%n.
+  Lemma n_impl_elim_l' {d i P Q R} : P ⊢{δ d, i} (Q → R) → P ∧ Q ⊢{δ d, i} R.
   Proof.
     move=> H. apply n_bysem=>/= >. apply bi.impl_elim_l'. by apply nin_sem in H.
   Qed.
 
   (** Laws for [∀] *)
   Lemma n_forall_intro {d i P A Ψ} :
-    (∀ a : A, δ d i (P, Ψ a)%n) → δ d i (P, ∀' Ψ)%n.
+    (∀ a : A, P ⊢{δ d, i} Ψ a) → P ⊢{δ d, i} ∀' Ψ.
   Proof.
     move=> ?. apply n_bysem=>/= >. apply bi.forall_intro=> ?. by apply nin_sem.
   Qed.
-  Lemma n_forall_elim {d i A Φ} {a : A} : δ d i (∀' Φ, Φ a)%n.
+  Lemma n_forall_elim {d i A Φ} {a : A} : ∀' Φ ⊢{δ d, i} Φ a.
   Proof.
     apply n_bysem=>/= >. apply (bi.forall_elim (Ψ := λ _, _)).
   Qed.
 
   (** Laws for [∃] *)
-  Lemma n_exist_intro {d i A Φ} {a : A} : δ d i (Φ a, ∃' Φ)%n.
+  Lemma n_exist_intro {d i A Φ} {a : A} : Φ a ⊢{δ d, i} ∃' Φ.
   Proof.
     apply n_bysem=>/= >. apply (bi.exist_intro (Ψ := λ a, ⟦ Φ a ⟧(_))).
   Qed.
   Lemma n_exist_elim {d i A Φ Q} :
-    (∀ a : A, δ d i (Φ a, Q)%n) → δ d i (∃' Φ, Q)%n.
+    (∀ a : A, Φ a ⊢{δ d, i} Q) → (∃' Φ) ⊢{δ d, i} Q.
   Proof.
     move=> ?. apply n_bysem=>/= >. apply bi.exist_elim=> ?. by apply nin_sem.
   Qed.
 
   (** Laws for [∗] *)
   Lemma n_sep_mono {d i P Q P' Q'} :
-    δ d i (P, Q) → δ d i (P', Q') → δ d i (P ∗ P', Q ∗ Q')%n.
+    P ⊢{δ d, i} Q → P' ⊢{δ d, i} Q' → P ∗ P' ⊢{δ d, i} Q ∗ Q'.
   Proof.
     move=> ??. apply n_bysem=>/= >. by apply bi.sep_mono; apply nin_sem.
   Qed.
-  Lemma n_True_sep_1 {d i P} : δ d i (P, True ∗ P)%n.
+  Lemma n_True_sep_1 {d i P} : P ⊢{δ d, i} True ∗ P.
   Proof. apply n_bysem=>/= >. apply uPred_primitive.True_sep_1. Qed.
-  Lemma n_True_sep_2 {d i P} : δ d i (True ∗ P, P)%n.
+  Lemma n_True_sep_2 {d i P} : True ∗ P ⊢{δ d, i} P.
   Proof. apply n_bysem=>/= >. apply uPred_primitive.True_sep_2. Qed.
-  Lemma n_sep_comm' {d i P Q} : δ d i (P ∗ Q, Q ∗ P)%n.
+  Lemma n_sep_comm' {d i P Q} : P ∗ Q ⊢{δ d, i} Q ∗ P.
   Proof. apply n_bysem=>/= >. apply bi.sep_comm'. Qed.
-  Lemma n_sep_assoc' {d i P Q R} : δ d i ((P ∗ Q) ∗ R, P ∗ (Q ∗ R))%n.
+  Lemma n_sep_assoc' {d i P Q R} : (P ∗ Q) ∗ R ⊢{δ d, i} P ∗ (Q ∗ R).
   Proof. apply n_bysem=>/= >. apply bi.sep_assoc'. Qed.
 
   (** Laws for [-∗] *)
-  Lemma n_wand_intro_r {d i P Q R} : δ d i (P ∗ Q, R)%n → δ d i (P, Q -∗ R)%n.
+  Lemma n_wand_intro_r {d i P Q R} : P ∗ Q ⊢{δ d, i} R → P ⊢{δ d, i} (Q -∗ R).
   Proof.
     move=> H. apply n_bysem=>/= >. apply bi.wand_intro_r. by apply nin_sem in H.
   Qed.
-  Lemma n_wand_elim_l' {d i P Q R} : δ d i (P, Q -∗ R)%n → δ d i (P ∗ Q, R)%n.
+  Lemma n_wand_elim_l' {d i P Q R} : P ⊢{δ d, i} (Q -∗ R) → P ∗ Q ⊢{δ d, i} R.
   Proof.
     move=> H. apply n_bysem=>/= >. apply bi.wand_elim_l'. by apply nin_sem in H.
   Qed.
 
   (** Laws for [□] *)
-  Lemma n_persistently_mono {d i P Q} : δ d i (P, Q) → δ d i (□ P, □ Q)%n.
+  Lemma n_persistently_mono {d i P Q} : P ⊢{δ d, i} Q → □ P ⊢{δ d, i} □ Q.
   Proof. move=> ?. apply n_bysem=>/= >. f_equiv. by apply nin_sem. Qed.
-  Lemma n_persistently_elim {d i P} : δ d i (□ P, P)%n.
+  Lemma n_persistently_elim {d i P} : □ P ⊢{δ d, i} P.
   Proof. apply n_bysem=>/= >. by iIntros. Qed.
-  Lemma n_persistently_idemp_2 {d i P} : δ d i (□ P, □ □ P)%n.
+  Lemma n_persistently_idemp_2 {d i P} : □ P ⊢{δ d, i} □ □ P.
   Proof. apply n_bysem=>/= >. by iIntros. Qed.
-  Lemma n_persistently_forall_2 {d i A Φ} : δ d i (∀ a : A, □ Φ a, □ ∀' Φ)%n.
+  Lemma n_persistently_forall_2 {d i A Φ} : (∀ a : A, □ Φ a) ⊢{δ d, i} □ ∀' Φ.
   Proof. apply n_bysem=>/= >. by iIntros "#? !#" (?). Qed.
-  Lemma n_persistently_exist_1 {d i A Φ} : δ d i (□ ∃' Φ, ∃ a : A, □ Φ a)%n.
+  Lemma n_persistently_exist_1 {d i A Φ} : □ ∃' Φ ⊢{δ d, i} ∃ a : A, □ Φ a.
   Proof. apply n_bysem=>/= >. iDestruct 1 as (a) "#?". by iExists a. Qed.
-  Lemma n_persistently_and_sep_l_1 {d i P Q} : δ d i (□ P ∧ Q, □ P ∗ Q)%n.
+  Lemma n_persistently_and_sep_l_1 {d i P Q} : □ P ∧ Q ⊢{δ d, i} □ P ∗ Q.
   Proof. apply n_bysem=>/= >. iIntros "[#? ?]". by iSplit. Qed.
 
   (** Laws for [■] *)
-  Lemma n_plainly_mono {d i P Q} : δ d i (P, Q) → δ d i (■ P, ■ Q)%n.
+  Lemma n_plainly_mono {d i P Q} : P ⊢{δ d, i} Q → ■ P ⊢{δ d, i} ■ Q.
   Proof. move=> ?. apply n_bysem=>/= >. f_equiv. by apply nin_sem. Qed.
-  Lemma n_plainly_elim_persistently {d i P} : δ d i (■ P, □ P)%n.
+  Lemma n_plainly_elim_persistently {d i P} : ■ P ⊢{δ d, i} □ P.
   Proof. apply n_bysem=>/= >. by iIntros. Qed.
-  Lemma n_plainly_idemp_2 {d i P} : δ d i (■ P, ■ ■ P)%n.
+  Lemma n_plainly_idemp_2 {d i P} : ■ P ⊢{δ d, i} ■ ■ P.
   Proof. apply n_bysem=>/= >. by iIntros "#? !#". Qed.
-  Lemma n_plainly_forall_2 {d i A Φ} : δ d i (∀ a : A, ■ Φ a, ■ ∀' Φ)%n.
+  Lemma n_plainly_forall_2 {d i A Φ} : (∀ a : A, ■ Φ a) ⊢{δ d, i} ■ ∀' Φ.
   Proof. apply n_bysem=>/= >. by iIntros "#? !#" (?). Qed.
-  Lemma n_plainly_exist_1 {d i A Φ} : δ d i (■ ∃' Φ, ∃ a : A, ■ Φ a)%n.
+  Lemma n_plainly_exist_1 {d i A Φ} : ■ ∃' Φ ⊢{δ d, i} ∃ a : A, ■ Φ a.
   Proof. apply n_bysem=>/= >. iDestruct 1 as (a) "#?". by iExists a. Qed.
   Lemma n_persistently_impl_plainly {d i P Q} :
-    δ d i (■ P → □ Q, □ (■ P → Q))%n.
+    (■ P → □ Q) ⊢{δ d, i} □ (■ P → Q).
   Proof. apply n_bysem=>/= >. iIntros "#H !# #H'". iApply ("H" with "H'"). Qed.
-  Lemma n_plainly_impl_plainly {d i P Q} :
-    δ d i (■ P → ■ Q, ■ (■ P → Q))%n.
+  Lemma n_plainly_impl_plainly {d i P Q} : (■ P → ■ Q) ⊢{δ d, i} ■ (■ P → Q).
   Proof. apply n_bysem=>/= >. iIntros "#H !# #H'". iApply ("H" with "H'"). Qed.
 
   (** Laws for [|==>] *)
-  Lemma n_bupd_mono {d i P Q} : δ d i (P, Q) → δ d i (|==> P, |==> Q)%n.
+  Lemma n_bupd_mono {d i P Q} : P ⊢{δ d, i} Q → (|==> P) ⊢{δ d, i} |==> Q.
   Proof. move=> ?. apply n_bysem=>/= >. apply bupd_mono. by apply nin_sem. Qed.
-  Lemma n_bupd_intro {d i P} : δ d i (P, |==> P)%n.
+  Lemma n_bupd_intro {d i P} : P ⊢{δ d, i} |==> P.
   Proof. apply n_bysem=>/= >. apply bupd_intro. Qed.
-  Lemma n_bupd_trans {d i P} : δ d i (|==> |==> P, |==> P)%n.
+  Lemma n_bupd_trans {d i P} : (|==> |==> P) ⊢{δ d, i} |==> P.
   Proof. apply n_bysem=>/= >. apply bupd_trans. Qed.
-  Lemma n_bupd_frame_r {d i P Q} : δ d i ((|==> P) ∗ Q, |==> P ∗ Q)%n.
+  Lemma n_bupd_frame_r {d i P Q} : (|==> P) ∗ Q ⊢{δ d, i} |==> P ∗ Q.
   Proof. apply n_bysem=>/= >. apply bupd_frame_r. Qed.
-  Lemma n_bupd_plainly {d i P} : δ d i (|==> ■ P, ■ P)%n.
+  Lemma n_bupd_plainly {d i P} : (|==> ■ P) ⊢{δ d, i} ■ P.
   Proof. apply n_bysem=>/= >. by iIntros ">?". Qed.
 
   (** Laws for [|={_,_}=>] *)
   Lemma n_fupd_mask_subseteq {d i E E' P} :
-    E' ⊆ E → δ d i (P, |={E,E'}=> |={E',E}=> True)%n.
+    E' ⊆ E → P ⊢{δ d, i} |={E,E'}=> |={E',E}=> True.
   Proof.
     move=> ?. apply n_bysem=>/= >. iIntros "_". by iMod fupd_mask_subseteq.
   Qed.
   Lemma n_except_0_fupd {d i E E' P} :
-    δ d i (◇ (|={E,E'}=> P), |={E,E'}=> P)%n.
+    ◇ (|={E,E'}=> P) ⊢{δ d, i} |={E,E'}=> P.
   Proof.
     apply n_bysem=>/= >. rewrite nintp_fp_nintp/=. by iDestruct 1 as "[>?|?]".
   Qed.
   Lemma n_fupd_mono {d i E E' P Q} :
-    δ d i (P, Q) → δ d i (|={E,E'}=> P, |={E,E'}=> Q)%n.
+    P ⊢{δ d, i} Q → (|={E,E'}=> P) ⊢{δ d, i} |={E,E'}=> Q.
   Proof.
     move=> ?. apply n_bysem=>/= >. apply fupd_mono. by apply nin_sem.
   Qed.
   Lemma n_fupd_trans {d i E E' E'' P} :
-    δ d i (|={E,E'}=> |={E',E''}=> P, |={E,E''}=> P)%n.
+    (|={E,E'}=> |={E',E''}=> P) ⊢{δ d, i} |={E,E''}=> P.
   Proof. apply n_bysem=>/= >. apply fupd_trans. Qed.
   Lemma n_fupd_mask_frame_r' {d i E E' Ef P} :
-    E ## Ef → δ d i (|={E,E'}=> ⌜E' ## Ef⌝ → P, |={E ∪ Ef,E' ∪ Ef}=> P)%n.
+    E ## Ef → (|={E,E'}=> ⌜E' ## Ef⌝ → P) ⊢{δ d, i} |={E ∪ Ef,E' ∪ Ef}=> P.
   Proof. move=> ?. apply n_bysem=>/= >. by apply fupd_mask_frame_r'. Qed.
   Lemma n_fupd_frame_r {d i E E' P Q} :
-    δ d i ((|={E,E'}=> P) ∗ Q, |={E,E'}=> P ∗ Q)%n.
+    (|={E,E'}=> P) ∗ Q ⊢{δ d, i} |={E,E'}=> P ∗ Q.
   Proof. apply n_bysem=>/= >. apply fupd_frame_r. Qed.
 
   (** Laws for [▷] *)
-  Lemma n_later_mono {d i P Q} : δ d i (P, Q) → δ d i (▷{nil} P, ▷{nil} Q)%n.
+  Lemma n_later_mono {d i P Q} : P ⊢{δ d, i} Q → ▷{nil} P ⊢{δ d, i} ▷{nil} Q.
   Proof.
     move=> ?. apply n_bysem=>/= >. f_equiv. rewrite !nintp_fp_nintp.
     by apply nin_sem.
   Qed.
-  Lemma n_later_intro {d i} {P : nPropL (;ᵞ)} : δ d i (P, ▷{nil} P)%n.
+  Lemma n_later_intro {d i} {P : nPropL (;ᵞ)} : P ⊢{δ d, i} ▷{nil} P.
   Proof.
     apply n_bysem=>/= >. rewrite nintp_fp_nintp. apply bi.later_intro.
   Qed.
   Lemma n_later_forall_2 {d i A} {Φ : A → nPropL (;ᵞ)} :
-    δ d i (∀ a, ▷{nil} Φ a, ▷{nil} ∀' Φ)%n.
+    (∀ a, ▷{nil} Φ a) ⊢{δ d, i} ▷{nil} ∀' Φ.
   Proof.
     apply n_bysem=>/= >. setoid_rewrite nintp_fp_nintp=>/=.
     apply bi.later_forall_2.
   Qed.
   Lemma n_later_exist_except_0 {d i A} {Φ : A → nPropL (;ᵞ)} :
-    δ d i (▷{nil} ∃ a, Φ a, ◇ (∃ a, ▷{nil} Φ a))%n.
+    ▷{nil} (∃ a, Φ a) ⊢{δ d, i} ◇ (∃ a, ▷{nil} Φ a).
   Proof.
     apply n_bysem=>/= >. setoid_rewrite nintp_fp_nintp=>/=.
     apply bi.later_exist_false.
   Qed.
   Lemma n_later_sep_1 {d i} {P Q : nPropL (;ᵞ)} :
-    δ d i (▷{nil} (P ∗ Q), ▷{nil} P ∗ ▷{nil} Q)%n.
+    ▷{nil} (P ∗ Q) ⊢{δ d, i} ▷{nil} P ∗ ▷{nil} Q.
   Proof.
     apply n_bysem=>/= >. rewrite !nintp_fp_nintp/=. apply bi.later_sep_1.
   Qed.
   Lemma n_later_sep_2 {d i} {P Q : nPropL (;ᵞ)} :
-    δ d i (▷{nil} P ∗ ▷{nil} Q, ▷{nil} (P ∗ Q))%n.
+    ▷{nil} P ∗ ▷{nil} Q ⊢{δ d, i} ▷{nil} (P ∗ Q).
   Proof.
     apply n_bysem=>/= >. rewrite !nintp_fp_nintp/=. apply bi.later_sep_2.
   Qed.
   Lemma n_later_false_em {d i} {P : nPropL (;ᵞ)} :
-    δ d i (▷{nil} P, ◇ (▷ False → P))%n.
+    ▷{nil} P ⊢{δ d, i} ◇ (▷ False → P).
   Proof.
     apply n_bysem=>/= >. rewrite !nintp_fp_nintp/=. apply bi.later_false_em.
   Qed.
   Lemma n_later_persistently_1 {d i} {P : nPropL (;ᵞ)} :
-    δ d i (▷{nil} □ P, □ ▷{nil} P)%n.
+    ▷{nil} □ P ⊢{δ d, i} □ ▷{nil} P.
   Proof.
     apply n_bysem=>/= >. rewrite !nintp_fp_nintp/=. iIntros "#? !#". by iNext.
   Qed.
   Lemma n_later_persistently_2 {d i} {P : nPropL (;ᵞ)} :
-    δ d i (□ ▷{nil} P, ▷{nil} □ P)%n.
+    □ ▷{nil} P ⊢{δ d, i} ▷{nil} □ P.
   Proof.
     apply n_bysem=>/= >. rewrite !nintp_fp_nintp/=. iIntros. by iNext.
   Qed.
   Lemma n_later_plainly_1 {d i} {P : nPropL (;ᵞ)} :
-    δ d i (▷{nil} ■ P, ■ ▷{nil} P)%n.
+    ▷{nil} ■ P ⊢{δ d, i} ■ ▷{nil} P.
   Proof.
     apply n_bysem=>/= >. rewrite !nintp_fp_nintp/=. iIntros "#? !#". by iNext.
   Qed.
   Lemma n_later_plainly_2 {d i} {P : nPropL (;ᵞ)} :
-    δ d i (■ ▷{nil} P, ▷{nil} ■ P)%n.
+    ■ ▷{nil} P ⊢{δ d, i} ▷{nil} ■ P.
   Proof.
     apply n_bysem=>/= >. rewrite !nintp_fp_nintp/=. iIntros. by iNext.
   Qed.
-  Lemma n_löb {d i P} : δ d i ((▷{nil} P → P), P)%n.
+  Lemma n_löb {d i P} : (▷{nil} P → P) ⊢{δ d, i} P.
   Proof. apply n_bysem=>/= >. rewrite nintp_fp_nintp/=. apply bi.löb. Qed.
 
   (** Laws for [∀:] *)
   Lemma n_n_forall_intro {d i V P Q} :
-    (∀ Φ, δ d i (P, nsubst Q Φ)%n) → δ d i (P, ∀: V, Q)%n.
+    (∀ Φ, P ⊢{δ d, i} nsubst Q Φ) → P ⊢{δ d, i} ∀: V, Q.
   Proof.
     move=> ?. apply n_bysem=>/= >. apply bi.forall_intro=> ?.
     rewrite rew_eq_hwf. by apply nin_sem.
   Qed.
-  Lemma n_n_forall_elim {d i V P Φ} : δ d i (∀: V, P, nsubst P Φ)%n.
+  Lemma n_n_forall_elim {d i V P Φ} : (∀: V, P) ⊢{δ d, i} nsubst P Φ.
   Proof.
     apply n_bysem=>/= >. setoid_rewrite rew_eq_hwf.
     apply (bi.forall_elim (Ψ := λ _, _)).
   Qed.
 
   (** Laws for [∃:] *)
-  Lemma n_n_exist_intro {d i V P Φ} : δ d i (nsubst P Φ, ∃: V, P)%n.
+  Lemma n_n_exist_intro {d i V P Φ} : nsubst P Φ ⊢{δ d, i} ∃: V, P.
   Proof.
     apply n_bysem=>/= >. setoid_rewrite rew_eq_hwf.
     apply (bi.exist_intro (Ψ := λ Φ, ⟦ nsubst _ Φ ⟧(_))).
   Qed.
   Lemma n_n_exist_elim {d i V P Q} :
-    (∀ Φ, δ d i (nsubst P Φ, Q)) → δ d i (∃: V, P, Q)%n.
+    (∀ Φ, nsubst P Φ ⊢{δ d, i} Q) → (∃: V, P) ⊢{δ d, i} Q.
   Proof.
     move=> ?. apply n_bysem=>/= >. apply bi.exist_elim=> ?.
     rewrite rew_eq_hwf. by apply nin_sem.
@@ -271,23 +270,23 @@ Section nola.
 
   (** Laws for [rec:ˢ] *)
   Lemma n_recs_unfold {d i A Φ} {a : A} :
-    δ d i (rec:ˢ' Φ a, nlarge (nsubst (Φ a) (rec:ˢ' Φ)))%n.
+    rec:ˢ' Φ a ⊢{δ d, i} nlarge (nsubst (Φ a) (rec:ˢ' Φ)%n).
   Proof. apply n_bysem=>/= >. by rewrite rew_eq_hwf nintp_nlarge. Qed.
   Lemma n_recs_fold {d i A Φ} {a : A} :
-    δ d i (nlarge (nsubst (Φ a) (rec:ˢ' Φ)), rec:ˢ' Φ a)%n.
+    nlarge (nsubst (Φ a) (rec:ˢ'%n Φ)) ⊢{δ d, i} rec:ˢ' Φ a.
   Proof. apply n_bysem=>/= >. by rewrite nintp_nlarge rew_eq_hwf. Qed.
 
   (** Laws for [rec:ˡ] *)
   Lemma n_recl_unfold {d i A Φ} {a : A} :
-    δ d i (rec:ˡ' Φ a, nsubst (Φ a) (rec:ˡ' Φ))%n.
+    rec:ˡ' Φ a ⊢{δ d, i} nsubst (Φ a) (rec:ˡ' Φ)%n.
   Proof. apply n_bysem=>/= >. by rewrite rew_eq_hwf. Qed.
   Lemma n_recl_fold {d i A Φ} {a : A} :
-    δ d i (nsubst (Φ a) (rec:ˡ' Φ), rec:ˡ' Φ a)%n.
+    nsubst (Φ a) (rec:ˡ' Φ)%n ⊢{δ d, i} rec:ˡ' Φ a.
   Proof. apply n_bysem=>/= >. by rewrite rew_eq_hwf. Qed.
 
   (** Laws for [!ᵘˢ] *)
-  Lemma n_subus_unfold {d i P} : δ d i (!ᵘˢ P, nlarge P)%n.
+  Lemma n_subus_unfold {d i P} : !ᵘˢ P ⊢{δ d, i} nlarge P.
   Proof. apply n_bysem=>/= >. by rewrite nintpS_nintp_nlarge. Qed.
-  Lemma n_subus_fold {d i P} : δ d i (nlarge P, !ᵘˢ P)%n.
+  Lemma n_subus_fold {d i P} : nlarge P ⊢{δ d, i} !ᵘˢ P.
   Proof. apply n_bysem=>/= >. by rewrite nintpS_nintp_nlarge. Qed.
 End nola.
